AVM/Class/Translation/Logics.lean
@@ -3,21 +3,6 @@ import AVM.Message
 import AVM.Logic
 import AVM.Ecosystem
 
-namespace AVM.Logic
-
-def classLogicRef {lab : Ecosystem.Label} (classId : lab.ClassId) : Anoma.LogicRef :=
-  classId.label.logicRef
-
-def trivialLogicRef : Anoma.LogicRef := Anoma.LogicRef.mk "Anoma.TrivialLogic"
-
-def trivialLogic : Anoma.Logic :=
-  { reference := trivialLogicRef,
-    function := fun _ => true }
-
-abbrev builtinLogics : List Anoma.Logic := [trivialLogic]
-
-end AVM.Logic
-
 namespace AVM.Program
 
 structure MessageValue (lab : Ecosystem.Label) where
@@ -78,7 +63,7 @@ def checkMessageResourceValues {lab : Ecosystem.Label} (vals : List (Program.Mes
   List.all₂
     (fun val res =>
       let try msg : Message lab := Message.fromResource res
-      msg.id == val.id && msg.args === val.args && msg.logicRef == val.logicRef)
+      msg.data.id == val.id && msg.data.args === val.args)
     vals
     resMsgs
 
@@ -93,16 +78,15 @@ def MultiMethod.Message.logicFun
   (msg : Message lab)
   (args : Logic.Args)
   : Bool :=
-  check h : msg.id == .multiMethodId multiId
-  let fargs : multiId.Args.type := cast (by simp! [eq_of_beq h]) msg.args
+  check h : msg.data.id == .multiMethodId multiId
+  let fargs : multiId.Args.type := cast (by simp! [eq_of_beq h]) msg.data.args
   let consumedResObjs := Logic.selectObjectResources args.consumed
   let createdResObjs := Logic.selectObjectResources args.created
   let argsConsumedSelves := consumedResObjs.take multiId.numObjectArgs
   let try argsConsumedObjects : multiId.Selves := Label.MultiMethodId.ConsumedToSelves argsConsumedSelves
+  check method.invariant msg argsConsumedObjects fargs
   let prog := method.body argsConsumedObjects fargs
-  let signatures := cast (by grind only) msg.signatures
-  check method.invariant argsConsumedObjects fargs signatures
-  let try vals : prog.params.Product := tryCast msg.vals
+  let try vals : prog.params.Product := tryCast msg.data.vals
   let res : MultiMethodResult multiId := prog.value vals
   let valsObjs := prog.objects vals
   let fetchedObjValues := valsObjs.map (·.toObjectValue)
@@ -160,11 +144,10 @@ private def Constructor.Message.logicFun
   (msg : Message lab)
   (args : Logic.Args)
   : Bool :=
-  check h : msg.id == .classMember (Label.MemberId.constructorId constrId)
-  let argsData : constrId.Args.type := cast (by simp! [eq_of_beq h]) msg.args
-  let signatures : constrId.Signatures argsData := cast (by grind only) msg.signatures
+  check h : msg.data.id == .classMember (Label.MemberId.constructorId constrId)
+  let argsData : constrId.Args.type := cast (by simp! [eq_of_beq h]) msg.data.args
   let body := constr.body argsData
-  let try vals : body.params.Product := tryCast msg.vals
+  let try vals : body.params.Product := tryCast msg.data.vals
   let newObjData := body.value vals
   let consumedResObjs := Logic.selectObjectResources args.consumed
   let createdResObjs := Logic.selectObjectResources args.created
@@ -182,7 +165,7 @@ private def Constructor.Message.logicFun
     && Logic.checkResourcesEphemeral [consumedObjRes]
     && Logic.checkResourcesPersistent createdResObjs
     && Logic.checkResourcesPersistent consumedFetchedResObjs
-    && constr.invariant argsData signatures
+    && constr.invariant msg argsData
 
 /-- Creates a message logic function for a given destructor. -/
 private def Destructor.Message.logicFun
@@ -193,16 +176,15 @@ private def Destructor.Message.logicFun
   (msg : Message lab)
   (args : Logic.Args)
   : Bool :=
-  check h : msg.id == .classMember (Label.MemberId.destructorId destructorId)
-  let argsData := cast (by simp! [eq_of_beq h]) msg.args
-  let signatures : destructorId.Signatures argsData := cast (by grind only) msg.signatures
+  check h : msg.data.id == .classMember (Label.MemberId.destructorId destructorId)
+  let argsData := cast (by simp! [eq_of_beq h]) msg.data.args
   let consumedResObjs := Logic.selectObjectResources args.consumed
   let createdResObjs := Logic.selectObjectResources args.created
   let! (selfRes :: _) := consumedResObjs
   let! (createdResObj :: createdFetchedResObjs) := createdResObjs
   let try selfObj : Object classId := Object.fromResource selfRes
   let body := destructor.body selfObj argsData
-  let try vals : body.params.Product := tryCast msg.vals
+  let try vals : body.params.Product := tryCast msg.data.vals
   let messageValues := Program.messageValues body vals
   let createdResMsgs := Logic.selectMessageResources args.created
   let valsObjs := body.objects vals
@@ -214,7 +196,7 @@ private def Destructor.Message.logicFun
     && Logic.checkResourcesPersistent consumedResObjs
     && Logic.checkResourcesEphemeral [createdResObj]
     && Logic.checkResourcesPersistent createdFetchedResObjs
-    && destructor.invariant selfObj argsData signatures
+    && destructor.invariant msg selfObj argsData
 
 private def Method.Message.logicFun
   {lab : Ecosystem.Label}
@@ -224,16 +206,15 @@ private def Method.Message.logicFun
   (msg : Message lab)
   (args : Logic.Args)
   : Bool :=
-  check h : msg.id == .classMember (Label.MemberId.methodId methodId)
-  let argsData : methodId.Args.type := cast (by simp! [eq_of_beq h]) msg.args
+  check h : msg.data.id == .classMember (Label.MemberId.methodId methodId)
+  let argsData : methodId.Args.type := cast (by simp! [eq_of_beq h]) msg.data.args
   let consumedResObjs := Logic.selectObjectResources args.consumed
   let createdResObjs := Logic.selectObjectResources args.created
   let! (selfRes :: _) := consumedResObjs
   let try selfObj : Object classId := Object.fromResource selfRes
   let body := method.body selfObj argsData
-  let try vals : body.params.Product := tryCast msg.vals
-  let signatures : methodId.Signatures argsData := cast (by grind only) msg.signatures
-  check method.invariant selfObj argsData signatures
+  let try vals : body.params.Product := tryCast msg.data.vals
+  check method.invariant msg selfObj argsData
   let createdObject : Object classId := body |>.value vals
   let messageValues := Program.messageValues body vals
   let createdResMsgs := Logic.selectMessageResources args.created
@@ -314,8 +295,8 @@ private def logicFun
       -- Note: the success of the `try` below ensures that the message is "legal"
       -- for the consumed objects - it is from the same ecosystem
       let try msg : Message lab := Message.fromResource consumedMessageResource
-      self.uid ∈ msg.recipients
-      && Member.logicFun eco msg.id msg args
+      self.uid ∈ msg.data.recipients
+      && Member.logicFun eco msg.data.id msg args
 
 /-- The class logic that is the Resource Logic of each resource corresponding to
   an object of this class. -/
