SUMMARY.md
@@ -19,6 +19,7 @@ A high-level summary description of GOOSE v0.3.1. The description intentionally 
 		- [MultiMethod](#multimethod)
 		- [Class](#class)
 		- [Ecosystem](#ecosystem)
+		- [Authorization](#authorization)
 	- [AVM -\> RM translation](#avm---rm-translation)
 		- [Object](#object-1)
 			- [Resource data check](#resource-data-check)
@@ -204,11 +205,10 @@ Action sending the call messages:
   - `vals : Vals`. Message parameter values. The message parameters are object resources and generated random values that are used in the body of the call associated with the message. These need to be provided in the message, because the associated Resource Logic cannot fetch object resources from the Anoma system or generate new object identifiers.
   - `id : MessageId`. The message ID.
   - `args : id.Args`. The arguments of the message, where `id.Args` is the type of arguments based on the message id. The message arguments are the non-self arguments of the corresponding member or multi-method call.
-  - `data : Option MultiMethodData`. Extra data for multi-methods which contains the numbers of:
-    - disassembled selves,
-    - destroyed selves,
-    - constructed objects.
   - `recipients : List ObjectId`. The recipients of the message.
+  - `signatures : List Signature`. Authorization signatures for the message. Each signature consists of:
+    - public identifier of the signer,
+    - signature data: the message `id`, `args` and `vals` cryptographically signed with signer's private key.
 
 ### Constructor
 - `Class.Constructor` in `AVM/Class/Member.lean`
@@ -218,7 +218,7 @@ Action sending the call messages:
 	- `id : label.ConstructorId` determines the unique id of the constructor.
 	- `Args := label.ConstructorArgs id` is the type of constructor arguments.
 	- `body : Args -> Program ObjectData`. Constructor body, returning the object data for the object created by the constructor call.
-	- `invariant : Args -> Bool`. Extra constructor logic. The constructor message logic is a conjunction of auto-generated constructor logic and the extra constructor logic.
+	- `invariant : Message -> Args -> Bool`. Extra constructor logic. The constructor message logic is a conjunction of auto-generated constructor logic and the extra constructor logic.
 
 ### Destructor
 - `Class.Destructor` in `AVM/Class/Member.lean`
@@ -228,7 +228,7 @@ Action sending the call messages:
 	- `id : label.DestructorId` determines the unique id of the destructor.
 	- `Args := label.DestructorArgs id` is the type of destructor arguments excluding `self`.
 	- `body : (self : Object) -> Args -> Program Unit`. Destructor body program.
-	- `invariant : (self : Object) -> Args -> Bool`. Extra destructor logic. The destructor message logic is a conjunction of auto-generated destructor logic and the extra destructor logic.
+	- `invariant : Message -> (self : Object) -> Args -> Bool`. Extra destructor logic. The destructor message logic is a conjunction of auto-generated destructor logic and the extra destructor logic.
 
 ### Method
 - `Class.Method` in `AVM/Class/Member.lean`
@@ -238,7 +238,7 @@ Action sending the call messages:
 	- `id : label.MethodId` determines the unique id of the method.
 	- `Args := label.MethodArgs id` is the type of method arguments excluding `self`.
 	- `body : (self : Object) -> Args -> Program Object`. Method body program. The return value is the updated `self`.
-	- `invariant : (self : Object) -> Args -> Bool`. Extra method logic. The method message logic is a conjunction of auto-generated method logic and the extra method logic.
+	- `invariant : Message -> (self : Object) -> Args -> Bool`. Extra method logic. The method message logic is a conjunction of auto-generated method logic and the extra method logic.
 
 ### MultiMethod
 - `MultiMethod` in `AVM/Ecosystem/Member.lean`
@@ -253,7 +253,7 @@ Action sending the call messages:
 		- `destroyed : List Object`. List of destroyed selves. Destroyed object resources are balanced with automatically generated created ephemeral resources. The `destroyed` list must be a sublist of `selves`.
 		- `assembled : List Object`. List of assembled objects into which disassembled objects are transformed as a result of the multi-method call. It is the responsibility of the user to ensure that assembled object resources balance with the disassembled selves.
 		- `constructed : List Object`. List of constructed objects. Constructed object resources are balanced with automatically generated consumed ephemeral resources.
-	- `invariant : (selves : List Object) -> Args -> Bool`. Extra multi-method logic. The multi-method message logic is a conjunction of the auto-generated multi-method logic and the extra multi-method logic.
+	- `invariant : Message -> (selves : List Object) -> Args -> Bool`. Extra multi-method logic. The multi-method message logic is a conjunction of the auto-generated multi-method logic and the extra multi-method logic.
 - `selves : List Object` in `body` and `invariant` above is a list of `self` arguments - objects whose classes are described by `label.MultiMethodSelves id`.
 - `selves = disassembled ++ destroyed`.
 
@@ -274,6 +274,11 @@ Action sending the call messages:
 	- `label : Ecosystem.Label`. Unique ecosystem label.
 	- `classes : Set Class`. Classes in the ecosystem. A class is in exactly one ecosystem.
 	- `multiMethods : Set MultiMethod`. Multi-methods in the ecosystem. A multi-method is in exactly one ecosystem.
+
+### Authorization
+The GOOSE framework provides a function `checkSignature : Message -> PublicKey -> Bool` which checks that a given message was signed with the private key corresponding to a given public key. In other words, `checkSignature(msg, pubKey)` checks that decrypting `msg.signature` with `pubKey` yields (a digest of) `msg`.
+
+The `checkSignature` function can be used in invariants to perform authorization of the received messages.
 
 ## AVM -> RM translation
 
@@ -594,12 +599,18 @@ Multi-method message logic has access to RL arguments which contain the followin
 
 - `consumed : List Resource`. List of resources consumed in the transaction.
 - `created : List Resource`. List of resources created in the transaction.
-- `msgRes : Resource`. The resource of the method message `msg`, which contains the method call arguments `args` and the `data` field with the numbers of:
+- `msgRes : Resource`. The resource of the method message `msg`, which contains the method call arguments `args` and parameter values `vals`.
+
+For a given multi-method, the number `n` of `selves` is specified in the
+multi-method definition. We re-create the `selves` objects from the first `n`
+object resources in `consumed`.
+
+With `selves`, `args` and `vals`, we compute the result of of the multi-method. In this way, we obtain the numbers of:
   - disassembled selves,
   - destroyed selves,
   - constructed objects.
 
-For a given multi-method, we use the numbers stored in `msg.data` to partition the object resources in `consumed` into:
+We use the above numbers to partition the object resources in `consumed` into:
 
 - `disassembledSelves` list of persistent object resources corresponding to disassembled selves,
 - `destroyedSelves` list of persistent object resources corresponding to destroyed selves,
